![[Pasted image 20241020174119.png]]
![[Pasted image 20241020174201.png]]
![[Pasted image 20241020174213.png]]


Let me show you how to convert this First Order Logic sentence to CNF step by step.

1) First, let's write the English sentence in FOL:
   "Ravi likes all kind of food"
   Initial FOL: ∀x(Food(x) → Likes(Ravi, x))

2) Steps for CNF conversion:

   a) Eliminate implications (→):
   - Replace (P → Q) with (¬P ∨ Q)
   - ∀x(¬Food(x) ∨ Likes(Ravi, x))

   b) Move negations inward (not needed here as there are no negations to push in)

   c) Standardize variables (not needed here as we already have clear variable usage)

   d) Skolemization (not needed here as we don't have existential quantifiers)

   e) Drop universal quantifiers (implicit in CNF):
   - ¬Food(x) ∨ Likes(Ravi, x)

   f) Distribute AND over OR (not needed here as we don't have conjunctions)

Final CNF: ¬Food(x) ∨ Likes(Ravi, x)

The sentence is already in CNF because:
- It's a disjunction of literals
- All variables are implicitly universally quantified
- No implications remain
- No existential quantifiers exist
- No conjunctions need distribution

This is the simplest form of the sentence in CNF, representing "for every x, either x is not food OR Ravi likes x".


- another example:
### Example: Converting FOL to CNF

![[Pasted image 20241120231147.png]]
![[Pasted image 20241120231205.png]]
![[Pasted image 20241120231219.png]]
![[Pasted image 20241120231231.png]]
